\chapter{From processes to rewriting}

\section{}

\begin{equation*}
  \begin{aligned}
    \trproc{\spawn{P}{Q}} &= \trproc{P} \fuse \trproc{Q} \\
            \trproc{\fwd} &= \one
    \\
                         \trproc{\selectR{\kay}} &= \atmR{\kay} \\
    \trproc{\caseL[\ell \in L]{\ell => Q_{\ell}}} &= \bigwith_{\ell \in L}\bigl(\atmR{\ell} \limp \trproc{Q_{\ell}}\bigr)
    \\
    \trproc{\caseR[\ell \in L]{\ell => P_{\ell}}} &= \bigwith_{\ell \in L}\bigl(\trproc{P_{\ell}} \pmir \atmL{\ell}\bigr) \\
                         \trproc{\selectL{\kay}} &= \atmL{\kay}
  \end{aligned}
\end{equation*}

\begin{equation*}
  \begin{aligned}
    \trconf{\cnfe} &= \cnfe \\
    \trconf{\cnf_1 \cc \cnf_2} &= \trconf{\cnf_1} \oc \trconf{\cnf_2} \\
    \trconf{P} &= \trproc{P}
  \end{aligned}
\end{equation*}

\begin{inferences}
  \infer{\slof{\sctx |- A_1 \fuse A_2 : C}}{
    \slof{\sctx |- A_1 : A} & \slof{A |- A_2 : C}}
  \and
  \infer{\slof{A |- A : A}}{}
  \\
  \infer{\slof{\sctx |- A \fuse \selectR{\kay} : \plus*[sub=_{\ell \in L}]{\ell:A_{\ell}}}}{
    \text{($\kay \in L$)} & \slof{\sctx |- A : A_{\kay}}}
  \and
  \infer{\slof{\plus*[sub=_{\ell \in L}]{\ell:A_{\ell}} |- \bigwith_{\ell \in L} (\selectR{\ell} \limp A_{\ell}) : C}}{
    \multipremise{\ell \in L}{\slof{A_{\ell} |- A_{\ell} : C}}}
  \\
  \text{(etc...)}
  \\
  \infer{\slcof{\sctx |- \octx_1 \oc \octx_2 : \sctx''}}{
    \slcof{\sctx |- \octx_1 : \sctx'} & \slcof{\sctx' |- \octx_2 : \sctx''}}
  \and
  \infer{\slcof{\sctx |- \octxe : \sctx'}}{}
  \and
  \infer{\slcof{\sctx |- A : A}}{
    \slof{\sctx |- A : A}}
\end{inferences}

\footnote{Careful with the 0-ary forms because you could end up with $\slof{\zero |- \top : C}$ and \emph{also} $\slof{\sctx |- \top : \top}$.}

\begin{theorem}
  If $\slof{\sctx |- P : A}$, then $\slof{\sctx |- \trproc{P} : A}$.
  Similarly, if $\slcof{\sctx |- \cnf : \sctx'}$, then $\slcof{\sctx |- \trconf{\cnf} : \sctx'}$.
\end{theorem}

\begin{theorem}
  If $\slof{\sctx |- A : A}$, then $\trproc{P} = A$ for some process $P$ such that $\slof{\sctx |- P : A}$.
  Similarly, if $\slcof{\sctx |- \octx : \sctx'}$, then $\trconf{\cnf} = \octx$ for some configuration $\cnf$ such that $\slcof{\sctx |- \cnf : \sctx'}$.
\end{theorem}


\section{}

\begin{equation*}
  \begin{lgathered}
    \tr{\spawn{P}{Q}} = \up (\dn \tr{P} \fuse \dn \tr{Q}) \\
    \tr{\fwd} = \up \one
    \\
    \tr{\selectR{\kay}[P]} = \up (\dn \tr{P} \fuse \atmR{\kay}) \\
    \tr{\caseL[\ell \in L]{\ell => Q_{\ell}}} = \with_{\ell \in L}(\atmR{\ell} \limp \up \dn \tr{Q_{\ell}})
    \\
    \tr{\caseR[\ell \in L]{\ell => P_{\ell}}} = \with_{\ell \in L}(\up \dn \tr{P_{\ell}} \pmir \atmL{\ell}) \\
    \tr{\selectL{\kay}[Q]} = \up (\atmL{\kay} \fuse \dn \tr{Q})
  \end{lgathered}
\end{equation*}

\begin{equation*}
  \begin{tikzcd}
    \spawn{P}{Q} \rar["\text{small step}"] \dar[dash] & P \cc Q \dar[dash] \\
    \up (\dn \tr{P} \fuse \dn \tr{Q}) \rar["\text{big step}"] & \tr{P} \oc \tr{Q}
  \end{tikzcd}
\end{equation*}

\begin{equation*}
  \begin{tikzcd}
    \selectR{\kay}[P] \rar["\text{small step}"] \dar[dash] & P \cc \selectR{\kay} \dar[dash] \\
    \up (\dn \tr{P} \fuse \selectR{\kay}) \rar["\text{big step}"] & \tr{P} \oc \selectR{\kay}
  \end{tikzcd}
\end{equation*}

\begin{equation*}
  \begin{tikzcd}
    \spawn{P}{(\selectR{\kay}[Q])} \arrow["\text{big step}"]{rr} \dar[dash] & & P \cc Q \cc \selectR{\kay} \dar[dash] \\
    \up (\dn \tr{P} \fuse \dn \up (\dn \tr{Q} \fuse \selectR{\kay})) \rar["\text{big step}"] & \tr{P} \oc \up (\dn \tr{Q} \fuse \selectR{\kay}) \rar["\text{big step}"] & \tr{P} \oc \tr{Q} \oc \selectR{\kay}
  \end{tikzcd}
\end{equation*}

\subsection{}

\begin{equation*}
  \begin{tikzcd}
    \spawn{P}{(\selectR{\kay}[Q])} \arrow["\text{big step}"]{r} \dar[dash] & P \cc Q \cc \selectR{\kay} \dar[dash] \\
    \llceil P \rrceil \fuse (\llceil Q \rrceil \fuse \selectR{\kay}) \rar["\text{big step}"] & \llceil P \rrceil \oc \llceil Q \rrceil \oc \selectR{\kay}
  \end{tikzcd}
\end{equation*}

\begin{equation*}
  \begin{lgathered}
    \llceil \spawn{P}{Q} \rrceil = \llceil P \rrceil \fuse \llceil Q \rrceil \\
    \llceil \fwd \rrceil = \one
    \\
    \llceil \selectR{\kay}[P] \rrceil = \llceil P \rrceil \fuse \atmR{\kay} \\
    \llceil \caseL[\ell \in L]{\ell => Q_{\ell}} \rrceil = \dn \bigwith_{\ell \in L}(\atmR{\ell} \limp \up \llceil Q_{\ell} \rrceil)
    \\
    \llceil \caseR[\ell \in L]{\ell => P_{\ell}} \rrceil = \dn \bigwith_{\ell \in L}(\up \llceil P_{\ell} \rrceil \pmir \atmL{\ell}) \\
    \llceil \selectL{\kay}[Q] \rrceil = \atmL{\kay} \fuse \llceil Q \rrceil
  \end{lgathered}
\end{equation*}

\subsection{}

\NewDocumentCommand \trp { s m } { \IfBooleanF {#1} ( #2 \IfBooleanF {#1} ) ^{-} }
\NewDocumentCommand \trc { s m } { \IfBooleanF {#1} ( #2 \IfBooleanF {#1} ) ^{+} }

\begin{syntax*}
  Processes & P & \caseL[\ell \in L]{\ell => \cnf_{\ell}} \mid \caseR[\ell \in L]{\ell => \cnf_{\ell}} \mid \mathsf{conf}\:\cnf
  \\
  Configurations & \cnf & (\cnf_1 \cc \cnf_2) \mid \cnfe \mid \selectL{\kay} \mid \selectR{\kay} \mid \mathsf{proc}\:P
\end{syntax*}

\begin{equation*}
  \begin{lgathered}[t]
    \trc{\cnf_1 \cc \cnf_2} = \trc*{\cnf_1} \fuse \trc*{\cnf_2} \\
    \trc{\cnfe} = \one \\
    \trc{\selectL{\kay}} = \atmL{\kay} \\
    \trc{\selectR{\kay}} = \atmR{\kay} \\
    \trc{\mathsf{proc}\:P} = \dn \trp*{P}
  \end{lgathered}
  \qquad
  \begin{lgathered}[t]
    \trp{\caseL[\ell \in L]{\ell => \cnf_{\ell}}} = \bigwith_{\ell \in L}(\atmR{\ell} \limp \up \trc*{\cnf_{\ell}}) \\
    \trp{\caseR[\ell \in L]{\ell => \cnf_{\ell}}} = \bigwith_{\ell \in L}(\up \trc*{\cnf_{\ell}} \pmir \atmL{\ell}) \\
    \trp{\mathsf{conf}\:\cnf} = \up \trc*{\cnf}
  \end{lgathered}
\end{equation*}

%%% Local Variables:
%%% mode: latex
%%% TeX-master: "thesis"
%%% End:
